\documentclass[11pt,fleqn]{article}

% ==== 中文環境 ====
\usepackage{CJK}

%% === AMS 標準套件 ===
\usepackage{amsmath,amsfonts,amssymb,amsthm} % 數學符號

%% === Symbol ====
\usepackage{mathtools}
\usepackage{upgreek}
\usepackage{relsize} % 改大小
%\usepackage{cancel}	% 刪除線

%% === border ===
\usepackage[margin=1in]{geometry}

%% === TikZ 套件 ===
\usepackage{tikz,tkz-graph,tkz-berge} 

%% 
\setlength{\parindent}{0pt}
\setlength{\parskip}{5pt plus 1pt}
\setlength{\headheight}{13.6pt}
\newtheorem{theorem}{定理}

\newcommand{\CourseLogo}{
\hrule\begin{center}
\textsf{Analysis of Binary Search Trees Algorithms}
\end{center}\hrule \bigskip\bigskip 
}

\begin{document}

\CourseLogo

Insert keys: 6, 3, 2, 1, 5, 4 $\Rightarrow$

\input{bst-example1}

\begin{align*}
	\left\{\begin{matrix*}[l]
		X_n &:= \hbox{\# probes per \phantom{un}{\bf succ} search 
		(for {\sl internal\/} node) in $n$-node BST} \\
		Y_n &:= \hbox{\# probes per {\bf unsucc} search 
		(for {\sl external\/} node)\qquad\ {\tt "}}
	\end{matrix*}\right.
\end{align*}
\begin{align*}
	\left\{\begin{matrix*}[l]
	\mathbb{E}(X) &=\dfrac{1}{6} \left(1+2+3+3+4+4\right) &= \dfrac{17}{6} = \dfrac{6+I(T)}{6} \\
	\mathbb{E}(Y) &=\dfrac{1}{7} \left(4+4+3+4+4+3+1\right) &= \dfrac{23}{7} =\dfrac{E(T)}{7}
	\end{matrix*}\right.
\end{align*}
\begin{align*}
	\left\{\begin{matrix*}[l]
		I(T) &:= \mathlarger{\sum}\limits_{x :\;\text{int node of } T} \text{path length}(x) = 11\\
		E(T) &:= \mathlarger{\sum}\limits_{y :\;\text{ext node of } T} \text{path length}(y) = 23
	\end{matrix*}\right.
\end{align*}
\[
\mathbb{E}(X_6)={1\over6}
\Bigl[
 \bigl(1+\mathbb{E}(Y_0)\bigr)
+\bigl(1+\mathbb{E}(Y_1)\bigr)
+\cdots
+\bigl(1+\mathbb{E}(Y_4)\bigr)
+\bigl(1+\mathbb{E}(Y_5)\bigr)
\Bigr]
\]
\begin{align*}
	\text{Sample Spaces} = \left\{\begin{matrix*}[l]
		\Omega_{X_n} &= \left\{(x_1, x_2, \ldots, x_n; k) 
			\left|{\displaystyle
				(x_1, x_2, \ldots, x_n) \in S_n \atop
				1\; \le\; k\; \le\; n
			}\right. 
		\right\}, & |\Omega_{X_n}| = n!\,n \\
		\Omega_{Y_n} &= \left\{(x_1, x_2, \ldots, x_n; y)
	   		\left|{\displaystyle	
				(x_1, x_2, \ldots, x_n) \in S_n \atop
				y\; =\; 0.5, \; 1.5, \; \ldots, \; n.5
			}\right.
		\right\}, & |\Omega_{Y_n}| = (n+1)!
	\end{matrix*}\right. 
\end{align*}
\begin{eqnarray*}
S_n&=&\hbox{set of all permutations of }\{1,2,\ldots,n\},
\qquad\qquad|S_n| = n!\\
\Omega_{Y_n}&=& \bigl\{(x_1, x_2, \ldots, x_n; y)
	   		\;|\;(x_1, x_2, \ldots, x_n; y) \in S_{n+1}\bigr\}
	   		\quad \hbox{by re-numbering}	   		
\end{eqnarray*}
\begin{align*}
	\left\{\begin{matrix*}[l]
		\hbox{Dynamic model}&:\; n!\hbox{ trees;} \\
		\hbox{Static\qquad\ {\tt "}}&:\; \frac{1}{n+1}{2n\choose n}\hbox{ trees,\quad (BST $6,3,2,1,5,4\equiv 6,3,5,4,2,1$)}
	\end{matrix*}\right.
\end{align*}

\pagebreak
\begin{table}[!hb]
	\label{bst}
	\begin{tabular}{|c | c | c | c | c|}
		\hline
		n & 1 & 2 & 3 &
		\\ \hline
		$\mathbb{E}(X_n) = 2 \frac{n+1}{n} H_n - 3$ & 1 & $\frac{3}{2}$ & $\frac{17}{9}$ & $\cdots\!\!\!\phantom{{{1\over1}\over{1\over1}}}$ 
		\\ \hline
		$\mathbb{E}(Y_n) = 2 H_{n+1} - 2$ & 1 & $\frac{5}{3}$ & $\frac{13}{6}$ & $\cdots\!\!\!\phantom{{{1\over1}\over{1\over1}}}$ 
		\\ \hline
	\end{tabular}
\end{table}

\begin{description}
	\item[\framebox{$n=1$}]
		\qquad\input{bst-n1}
		\begin{align*}
			\left\{\begin{matrix*}[l]
			\mathbb{E}(X_1) &= \frac{1}{1} \left[1\right] &= 1 \\
			\mathbb{E}(Y_1) &= \frac{1}{2}\left[1+1\right] &= 1 			 \phantom{\Bigl]} \\
			\end{matrix*}\right.
		\end{align*}
	\item[\framebox{$n=2$}]
		\qquad\input{bst-n2}
		\begin{align*}
			\left\{\begin{matrix*}[l]
		\mathbb{E}(X_2) &= \frac{1}{2 \cdot 2!} \left[(1+2) + (1+2)\right] 
						&= \frac{3}{2} \\
		\mathbb{E}(Y_2) &= \frac{1}{3 \cdot 2!} \left[(1+2+2) + (2+2+1)\right] 
						&= \frac{5}{3} \phantom{\Bigl]}
			\end{matrix*}\right.
		\end{align*}
	\item[\framebox{$n=3$}]
		\qquad\input{bst-n3}
		\begin{align*}
			\left\{\begin{matrix*}[l]
			\mathbb{E}(X_3) &= \frac{1}{3 \cdot 3!} 
			\left[(1+2+3)+(1+2+3)+(1+2+2)+(\cdot)+(\cdot)+(\cdot) \right]
						&= \frac{17}{9} \\
			\mathbb{E}(Y_3) &= \frac{1}{4 \cdot 3!}
		\left[(1+2+3+3)+(1+3+3+2)+(2+2+2+2)+(\cdot)+(\cdot)+(\cdot) \right] 
						&= \frac{13}{6}  \phantom{\Bigl]}
			\end{matrix*}\right.
		\end{align*}
\end{description}

\pagebreak
\noindent{\bf Lemma 1.}
$n$-node binary tree $T$ has\\ 
\hbox{\qquad}(1) $2n$ edges,\\ 
\hbox{\qquad}(2) $n+1$ external nodes (leaves),\\
\hbox{\qquad}(3) $E(T)=I(T)+2n$. 

\noindent{\bf Lemma 2.} 
$\displaystyle\mathbb{E}(X_n)=1+\frac{1}{n}\sum\limits_{1\le k\le n} \mathbb{E}(Y_{k-1})$

\noindent{\bf Theorem 3.}
\begin{align*}
	\left\{\begin{matrix*}[l]
		\mathbb{E}(X_n) &= 2 \frac{n+1}{n} H_n - 3 &\approx 2 \ln n\phantom{\Bigl]} \\
		\mathbb{E}(Y_n) &= 2 H_{n+1} - 2 &\approx 2 \ln n
	\end{matrix*}\right.
\end{align*}
\noindent{\bf Proof:}
\begin{align*}
	\left\{\begin{matrix*}[l]
	\mathbb{E}(X_n)&= \sum\limits_{w \in \Omega_{X_n} } P(w) X_n(w) 
				= \sum\limits_{
						\substack{
						(x_1, \ldots, x_n) \in S_n \\ 
						1 \le k \le n
						}} 
					\frac{1}{n!\,n} X_n (x_1, \ldots, x_n ; k) \\
			&= \frac{1}{n!\,n} 
	\sum\limits_{(x_1, \ldots, x_n) \in S_n} \sum\limits_{1 \le k \le n} 
					X_n (x_1, \ldots, x_n ; k) \\
	&= \frac{1}{n!\,n} \sum\limits_{T} \bigl(n +I(T)\bigr)\\ 
				&= \frac{1}{n} 
			\Bigl[ n + \frac{1}{n!} \sum\limits_{T}I(T)\Bigr] && \text{(1)}\\
\mathbb{E}(Y_n) &= \frac{1}{(n+1)!}\sum\limits_{(x_1, \ldots, x_n) \in S_n}
		\sum\limits_{y = 0.5, \ldots, n.5} Y_n(x_1 , \ldots, x_n ; y) \\
			&= \frac{1}{(n+1)!} \sum\limits_{T}E(T)\\ 
	&=\frac{1}{(n+1)n!}\sum\limits_{T}\bigl(2n +I(T)\bigr) \\
	&= \frac{1}{n+1} \Bigl[2n + \frac{1}{n!} \sum\limits_{T} I(T)\Bigr]&& \text{(2)}
	\end{matrix*}\right.
\end{align*}

\noindent $(1)+(2)\qquad\quad\;\; \Rightarrow(n+1)\mathbb{E}(Y_n)= n\mathbb{E}(X_n)+n$

\noindent $\phantom{(1)}+ {\bf Lemma\ 2}\ \Rightarrow$
\begin{align*}
(n+1)\,\mathbb{E}(Y_n)&=\sum\limits_{1\le k\le n}\mathbb{E}(Y_{k-1})+2n&\\
-\,\bigl)\qquad n\,\mathbb{E}(Y_{n-1})
	&=\sum\limits_{1\le k\le n-1 \phantom{{1\over1}}}
		\!\!\!\mathbb{E}(Y_{k-1})+2(n-1)&\\
\hline
(n+1)\,\mathbb{E}(Y_n) &= (n+1)\,\mathbb{E}(Y_{n-1}) + 2 \phantom{\Bigl]}
\end{align*}
\begin{align*}
\Rightarrow
		\left\{\begin{matrix*}[l]		
		\mathbb{E}(Y_n) &=\mathbb{E}(Y_{n-1}) + \frac{2}{n+1} \\
		\mathbb{E}(Y_{n-1}) &=\mathbb{E}(Y_{n-2}) + \frac{2}{n} \\
			 & \vdots &\\
			\mathbb{E}(Y_2) &=\mathbb{E}(Y_1) + \frac{2}{3}\\
			\mathbb{E}(Y_1) &= \frac{2}{2}
\end{matrix*}\right.
\end{align*}
\begin{align*}
	\Rightarrow
		\left\{\begin{matrix*}[l]
			\mathbb{E}(Y_n) &= 2 H_{n+1} - 2 \phantom{\Bigl]} \\
			\mathbb{E}(X_n) &=\frac{n+1}{n}E(Y_{n})-1=2\frac{n+1}{n} H_n - 3
		\qquad\qquad\blacksquare
		\end{matrix*}\right.
\end{align*}

\noindent{\bf Lemma 2.} 
$\displaystyle\mathbb{E}(X_n)=1+\frac{1}{n}\sum\limits_{1\le k\le n} \mathbb{E}(Y_{k-1})$

\noindent{\bf Proof:}
\begin{align*}
\mathbb{E}(X_n) 
	&= \frac{1}{n!\,n} \sum\limits_{(x_1, \ldots, x_n)} 
		\sum_{1 \le k \le n} X_n (x_1, \ldots, x_n ; k) \\
	&= \frac{1}{n!\,n} \sum\limits_{(x_1, \ldots, x_n) \in S_n}
		\sum\limits_{1\le k\le n}\Bigl(1+Y_n(x_1,\ldots,x_{k-1} ; k)\Bigl)\\
	&= 1 + \frac{1}{n!\,n} \sum\limits_{1 \le k \le n}
		\sum\limits_{(x_1, \ldots, x_{k}) \in S_k} 
			n \cdots (k+1) Y_{k-1} (x_1, \ldots, x_{k-1}; x_k) \\
	&= 1 + \frac{1}{n} \sum\limits_{1 \le k \le n}
		\biggl[\frac{1}{k!}\sum\limits_{(x_1, \ldots, x_{k}) \in S_k} 
			Y_{k-1} (x_1, \ldots, x_{k-1}; x_k)\biggr] \\
	&= 1 + \frac{1}{n} \sum\limits_{1 \le k \le n}\mathbb{E}(Y_{k-1})
	\qquad\qquad\blacksquare
\end{align*}

\end{document}